Changed the order handling of fexp2exp to make it work correctly. As it is, f_apply can be looked at as applying arguments in order from left to right, which might feel more familiar.
Added some auxiliary lemmas to help with the case for f_apply in the proof
of soundness.

FEV_Definitions.v
@@ -16,8 +16,8 @@ Fixpoint fexp2exp (e:fexp) : exp :=
   | f_new cn => e_new cn nil                  (* New 'base' *)
   | f_apply e1 e2 =>                          (* Method/New application *)
     match fexp2exp e1 with
-    | e_new cn al => e_new cn ((fexp2exp e2)::al)
-    | e_meth e mn al => e_meth e mn ((fexp2exp e2)::al)
+    | e_new cn al => e_new cn (al ++ (fexp2exp e2)::nil)
+    | e_meth e mn al => e_meth e mn (al ++ (fexp2exp e2)::nil)
     | e1 => e1 (* This case should never occur; it's malformed *)
     end
   end.
