FEV_Properties.v
@@ -2,7 +2,7 @@ Require Import Metatheory.
 Require Import FJ_Definitions.
 Require Import FEV_Definitions.
 
-Theorem decomp_no_apply:
+Lemma decomp_no_apply:
   forall (e1 e2 e3 e4:fexp), fst (decomp (f_apply e1 e2)) <> f_apply e3 e4.
 Proof.
   intro. induction e1; intros.
@@ -12,6 +12,46 @@ Proof.
   - simpl. discriminate.
   - apply IHe1_1.
 Qed.
+
+Lemma apply_rev_args:
+  forall (e1 e2 h:fexp) (t:list fexp),
+    h::t = rev (snd (decomp (f_apply e1 e2))) -> e2 = h.
+Proof.
+  intros. simpl in H. rewrite rev_app_distr in H. simpl in H. injection H.
+  intros. symmetry. assumption.
+Qed.
+
+Lemma decomp_apply_meth:
+  forall (e1 e2 eb:fexp) (ps:list fexp) (mn:mname),
+    decomp (f_apply e1 e2) = (f_meth eb mn, ps ++ e2::nil) ->
+      fexp2exp (f_apply e1 e2) = e_meth (fexp2exp eb) mn (List.map fexp2exp (ps ++ e2::nil)).
+Proof.
+  intro. induction e1; intros.
+  - simpl. discriminate.
+  - simpl. discriminate.
+  - inversion H. subst. reflexivity.
+  - simpl. discriminate.
+  - simpl. destruct e1_1 eqn:De1_1.
+    + discriminate.
+    + discriminate.
+    + simpl in *. injection H. intros. subst. injection H. intros.
+      rewrite <- H1. simpl. reflexivity.
+    + discriminate.
+    + injection H. intros. admit.
+Admitted.
+
+Lemma decomp_apply_new:
+  forall (e1 e2:fexp) (ps:list fexp) (cn:cname),
+    decomp (f_apply e1 e2) = (f_new cn, ps) ->
+      fexp2exp (f_apply e1 e2) = e_new cn (List.map fexp2exp ps).
+Proof.
+  intro. induction e1.
+  - simpl. discriminate.
+  - simpl. discriminate.
+  - simpl. discriminate.
+  - intros. inversion H. subst. simpl. reflexivity.
+  - intros. simpl in H.
+Admitted.
 
 Theorem feval_sound:
   forall (e1 e2:fexp) (fct:fctable), feval e1 fct = Some e2 -> eval (fexp2exp e1) (fexp2exp e2).
@@ -49,10 +89,17 @@ Proof.
         apply eval_context with (EE:=EE') in H0.
         --  subst. assumption.
         --  rewrite HeqEE'. apply ec_new_args. rewrite HeqEE''. apply esc_head.
-      * subst. destruct (fst (decomp (f_apply f0_1 f0_2))) eqn:DD.
+      * destruct (fst (decomp (f_apply f0_1 f0_2))) eqn:DD.
         --  discriminate.
         --  discriminate.
-        --  admit.
+        --  destruct (snd (decomp (f_apply f0_1 f0_2))) eqn:PS.
+            ++  simpl in PS. apply app_eq_nil in PS. destruct PS. discriminate.
+            ++  remember (rev (snd (decomp (f_apply f0_1 f0_2)))) as RPS.
+                destruct RPS.
+                **  simpl in HeqRPS. rewrite rev_app_distr in HeqRPS.
+                    symmetry in HeqRPS. apply app_eq_nil in HeqRPS.
+                    destruct HeqRPS. discriminate.
+                **  apply apply_rev_args in HeqRPS as F0_2. admit.
         --  admit.
         --  apply decomp_no_apply in DD. exfalso. assumption.
     + admit.
